Finished CRC32 table generation function.

code/Yazi.CRC32Table.fst
@@ -2,12 +2,78 @@ module Yazi.CRC32Table
 
 module B = LowStar.Buffer
 module BV = FStar.BitVector
-module Spec = Spec.CRC32
+module CB = LowStar.ConstBuffer
+module Ghost = FStar.Ghost
+module HS = FStar.HyperStack
+module M = LowStar.Modifies
+module Math = FStar.Math.Lemmas
 module Seq = FStar.Seq
-module U8 = FStar.UInt8
 module U32 = FStar.UInt32
 
 open FStar.Tactics
+open LowStar.BufferOps
+open Spec.CRC32
+
+let rec logand_mask_aux (a: nat{a > 0}) (n: nat{n >= a}): Lemma
+  (requires (pow2 a) - 1 < pow2 n)
+  (ensures forall i. 
+    (i >= n - a ==> UInt.nth #n ((pow2 a) - 1) i == true) /\
+    (i < n - a ==> UInt.nth #n ((pow2 a) - 1) i == false)) =
+  if n = a then
+    ()
+  else begin
+    Math.Lemmas.pow2_le_compat (n - 1) a;
+    logand_mask_aux a (n - 1)
+  end
+
+#set-options "--z3rlimit 120 --z3seed 1"
+let large_table_val_aux
+  (i: U32.t{U32.v i < 256}) (nzeros: nat{nzeros > 0}) (p p' p'': U32.t): Lemma
+  (requires
+    poly_mod_u32 nzeros i == UInt.to_vec (U32.v p) /\
+    poly_mod_u32 8 (U32.logand p 0xFFul) == UInt.to_vec (U32.v p') /\
+    p'' == U32.shift_right p 8ul)
+  (ensures poly_mod_correct (nzeros + 8) i (U32.logxor p' p'')) =
+   let open U32 in
+   let vi = UInt.to_vec (v i) in
+   let vp = UInt.to_vec (v p) in
+   let vp' = UInt.to_vec (v p') in
+   let vp'' = UInt.to_vec (v p'') in
+   let vpand = UInt.to_vec (U32.v (U32.logand p 0xFFul)) in
+   logand_mask_aux 8 32;
+   assert(forall i.
+     i < 32 - 8 ==> Seq.index vpand i == false /\
+     i >= 32 - 8 ==> Seq.index vpand i == Seq.index vp i);
+   assert(vp' == poly_mod (zero_vec_l 8 vpand));
+
+   assert(forall i.
+     i >= 8 ==> Seq.index vp'' i == Seq.index vp (i - 8) /\
+     i < 8 ==> Seq.index vp'' i == false);
+   poly_mod_zero_suffix vp'' 8;
+   assert(vp'' == poly_mod (zero_vec_r 8 vp''));
+
+   assert(forall i. {:pattern Seq.index (zero_vec_l 8 vpand) i}
+     (i >= 40 - 8 ==> Seq.index (zero_vec_l 8 vpand) i == Seq.index vp (i - 8)) /\
+     (i < 40 - 8 ==> Seq.index (zero_vec_l 8 vpand) i == false));
+
+   assert(forall i. {:pattern Seq.index (zero_vec_r 8 vp'') i}
+     (i < 8 \/ i >= 32 ==> Seq.index (zero_vec_r 8 vp'') i == false) /\
+     (i >= 8 /\ i < 32 ==> Seq.index (zero_vec_r 8 vp'') i == Seq.index vp (i - 8)));
+
+   let sum = (zero_vec_l 8 vpand) +@ (zero_vec_r 8 vp'') in
+   assert(forall i. {:pattern Seq.index sum i}
+     (i < 8 ==> Seq.index sum i == false) /\
+     (i >= 8 ==> Seq.index sum i == Seq.index vp (i - 8)));
+   assert(Seq.equal sum (zero_vec_l 8 vp));
+   
+   poly_mod_add (zero_vec_l 8 vpand) (zero_vec_r 8 vp'');
+   assert(poly_mod sum == poly_mod (zero_vec_l 8 vp));
+
+   assert(vp' +@ vp'' == poly_mod (zero_vec_l 8 (poly_mod (zero_vec_l nzeros vi))));
+   poly_mod_zero_prefix (zero_vec_l nzeros vi) 8;
+   assert(vp' +@ vp'' == poly_mod (zero_vec_l 8 (zero_vec_l nzeros vi)));
+   zero_vec_l_app vi nzeros 8;
+   assert(vp' +@ vp'' == poly_mod (zero_vec_l (nzeros + 8) vi))
 
 let rec uint_one_vec (#n: nat{n > 0}) (v: UInt.uint_t n): Lemma
   (requires v == 1)
@@ -33,53 +99,52 @@ let mask_logor_status (#n: nat{n > 0}) (s: nat{s < n}) (mask v: UInt.uint_t n): 
     (j == n - 1 - s ==> UInt.nth (UInt.logor v mask) j == true)) =
   mask_bit_status s mask
 
-#set-options "--z3rlimit 120"
+#set-options "--z3rlimit 120 --z3seed 1"
 inline_for_extraction
 private let poly_mask (i: U32.t{(U32.v i) < 32}) (p: U32.t{
   let p' = U32.v p in
   let i' = U32.v i in
   forall j. {:pattern UInt.nth p' j}
     (j >= i' ==> UInt.nth p' j == false) /\
-    (j < i' ==> UInt.nth p' j == Seq.index Spec.gf2_polynomial32 (31 - j))
+    (j < i' ==> UInt.nth p' j == Seq.index gf2_polynomial32 j)
 }): Tot (res: U32.t{
   let res' = U32.v res in
   let i' = U32.v i in
   forall j. {:pattern UInt.nth res' j}
     (j > i' ==> UInt.nth res' j == false) /\
-    (j <= i' ==> UInt.nth res' j == Seq.index Spec.gf2_polynomial32 (31 - j))
+    (j <= i' ==> UInt.nth res' j == Seq.index gf2_polynomial32 j)
 }) =
   if i = 0ul || i = 6ul || i = 9ul || i = 10ul || i = 16ul || i = 20ul || i = 21ul ||
   i = 22ul || i = 24ul || i = 25ul || i = 27ul || i = 28ul || i = 30ul || i = 31ul then
   begin
     let open U32 in
-    let one = 1ul in
     let shift = 31ul -^ i in
-    let mask = one <<^ shift in
+    let mask = 1ul <<^ shift in
     let res = p |^ mask in
     
     mask_logor_status #32 (v shift) (v mask) (v p);
     assert(forall j. {:pattern UInt.nth (UInt.logor (v p) (v mask)) j}
       j <> (32 - 1 - v shift) ==>
       UInt.nth (UInt.logor (v p) (v mask)) j == UInt.nth (v p) j);
-    assert_norm(Seq.index Spec.gf2_polynomial32 (v shift) == true);
+    assert_norm(Seq.index gf2_polynomial32 (v i) == true);
     res
   end else
     p
 
-let rec calc_polynomial (i: U32.t{U32.v i < 32}) (p: U32.t{
+private let rec calc_polynomial (i: U32.t{U32.v i < 32}) (p: U32.t{
   let i' = U32.v i in
   let p' = U32.v p in
   forall j. {:pattern UInt.nth p' j}
     (j >= i' ==> UInt.nth p' j == false) /\
-    (j < i' ==> UInt.nth p' j == Seq.index Spec.gf2_polynomial32 (31 - j))
-}): Tot Spec.crc32_polynomial (decreases U32.v (U32.sub 32ul i)) =
+    (j < i' ==> UInt.nth p' j == Seq.index gf2_polynomial32 j)
+}): Tot crc32_polynomial (decreases U32.v (U32.sub 32ul i)) =
   let open U32 in
   let p' = poly_mask i p in
   if i = 31ul then p' else calc_polynomial (i +^ 1ul) p'
 
 #set-options "--ifuel 64 --fuel 64"
 inline_for_extraction
-let gen_polynomial _: Tot Spec.crc32_polynomial =
+let gen_polynomial _: Tot crc32_polynomial =
   assert(forall i. UInt.nth (U32.v 0ul) i == false) by (
     let _ = forall_intro () in
     norm [simplify]);
@@ -89,7 +154,7 @@ let gen_polynomial _: Tot Spec.crc32_polynomial =
 
 let poly_mod_head_zero (d: U32.t): Lemma
   (requires UInt.nth (U32.v d) 31 == false)
-  (ensures Spec.poly_mod_correct d (U32.shift_right d 1ul)) =
+  (ensures poly_mod_correct 1 d (U32.shift_right d 1ul)) =
   ()
 
 let bv_one_aux (#n: nat{n > 0}) (v: BV.bv_t n): Lemma
@@ -113,29 +178,30 @@ let logand_aux (#n: nat{n > 0}) (d: UInt.uint_t n): Lemma
   end else
     ()
 
-let poly_xor_aux (d: U32.t) (p: Spec.crc32_polynomial): Lemma
+let poly_xor_aux (d: U32.t) (p: crc32_polynomial): Lemma
   (ensures forall i. {:pattern UInt.nth (U32.v (U32.logxor d p)) i}
     UInt.nth (U32.v (U32.logxor d p)) i ==
-    Seq.index (Spec.poly_xor (UInt.to_vec (U32.v (Spec.u32_rev d)))) (31 - i)) = ()
+    Seq.index (poly_xor (UInt.to_vec (U32.v d))) i) = ()
 
-#set-options "--z3rlimit 120"
-let poly_xor_poly_mod (d: U32.t) (p: Spec.crc32_polynomial): Lemma
+#set-options "--z3rlimit 120 --z3seed 1"
+let poly_xor_poly_mod (d: U32.t) (p: crc32_polynomial): Lemma
   (requires UInt.nth (U32.v d) 31 == true)
   (ensures
-    Spec.poly_mod (Spec.zero_vec_r 1 (UInt.to_vec (U32.v (Spec.u32_rev d)))) ==
-    Spec.poly_xor (UInt.to_vec (U32.v (Spec.u32_rev (U32.shift_right d 1ul))))) =
+    poly_mod (zero_vec_l 1 (UInt.to_vec (U32.v d))) ==
+    poly_xor (UInt.to_vec (U32.v (U32.shift_right d 1ul)))) =
   let open U32 in
-  let d' = UInt.to_vec (U32.v (Spec.u32_rev d)) in
-  let d'' = Spec.zero_vec_r 1 d' in
-  let d''' = UInt.to_vec (U32.v (Spec.u32_rev (d >>^ 1ul))) in
-  assert(Seq.head d'' == true);
-  assert(Seq.index d'' 32 == false);
-  assert(forall i. i < 32 ==> Seq.index d'' i == UInt.nth (v d) (31 - i));
-  assert(Seq.equal (Spec.poly_mod d'') (Spec.poly_xor #32 (Seq.tail d'')));
-  // assert(forall i. i < 31 ==> Seq.index d''' i == Seq.index d'' (i - 1));
-  admit()
-  
-let cell_xor (d: U32.t): Tot (res:U32.t{Spec.poly_mod_correct d res}) =
+  let d' = UInt.to_vec (U32.v d) in
+  let d'' = zero_vec_l 1 d' in
+  let d''' = UInt.to_vec (U32.v (d >>^ 1ul)) in
+  assert(Seq.last d'' == true);
+  assert(Seq.index d'' 0 == false);
+  assert(forall i. i > 1 ==> Seq.index d'' i == UInt.nth (v d) (i - 1));
+  assert(Seq.equal (poly_mod d'') (poly_xor #32 (unsnoc d'')));
+  assert(forall i. i <= 31 ==> Seq.index d''' i == Seq.index d'' i);
+  assert(Seq.equal d''' (unsnoc d''))
+
+inline_for_extraction
+private let cell_xor (d: U32.t): Tot (res:U32.t{poly_mod_correct 1 d res}) =
   let open U32 in
   let p = gen_polynomial () in
   let d' = d >>^ 1ul in
@@ -152,3 +218,80 @@ let cell_xor (d: U32.t): Tot (res:U32.t{Spec.poly_mod_correct d res}) =
     poly_mod_head_zero d;
     d'
   end
+
+let cell_xor_app (nzeros: nat{nzeros > 0}) (d res: U32.t): Lemma
+  (requires poly_mod_correct nzeros d res)
+  (ensures poly_mod_correct (nzeros + 1) d (cell_xor res)) =
+  let open U32 in
+  let d' = UInt.to_vec (v d) in
+  let d'' = zero_vec_l nzeros d' in
+  let res' = UInt.to_vec (U32.v res) in
+  calc (==) {
+    UInt.to_vec (U32.v (cell_xor res));
+    =={poly_mod_correct_eq 1 res (cell_xor res)}
+    poly_mod (zero_vec_l 1 res');
+    =={poly_mod_correct_eq nzeros d res}
+    poly_mod (zero_vec_l 1 (poly_mod d''));
+    =={poly_mod_zero_prefix d'' 1}
+    poly_mod (zero_vec_l 1 d'');
+    =={zero_vec_l_app d' nzeros 1}
+    poly_mod (zero_vec_l (nzeros + 1) d');
+  }
+
+private let rec calc_cell (m: Ghost.erased U32.t) (i: U32.t{U32.v i <= 7}) (d: U32.t{
+  let open U32 in
+  (v i < 7 ==> poly_mod_correct (v (7ul -^ i)) m d) /\
+  (v i == 7 ==> (v d) == (v m))
+}): Tot (res:U32.t{
+  poly_mod_correct 8 m res
+}) (decreases U32.v i) =
+  let open U32 in
+  if i <^ 7ul then cell_xor_app (v (7ul -^ i)) m d else ();
+  if i = 0ul then
+    cell_xor d
+  else
+    calc_cell m (i -^ 1ul) (cell_xor d)
+
+private let rec gen_8bit_table
+  (i: U32.t{U32.v i <= 255})
+  (buf: table_buf):
+  ST.Stack unit
+  (decreases 255 - U32.v i)
+  (requires fun h -> sub_table_correct (U32.v i) 8 h buf)
+  (ensures fun h0 _ h1 -> M.modifies (B.loc_buffer buf) h0 h1 /\ table_correct 8 h1 buf) =
+  let open U32 in
+  buf.(i) <- calc_cell i 7ul i;
+  if i <^ 255ul then gen_8bit_table (i +^ 1ul) buf else ()
+
+private let rec gen_large_table
+  (nzeros: Ghost.erased nat{nzeros > 0})
+  (i: U32.t{U32.v i <= 255})
+  (t8 tp buf: table_buf):
+  ST.Stack unit
+    (decreases 255 - U32.v i)
+    (requires fun h ->
+      B.disjoint buf t8 /\
+      B.disjoint buf tp /\
+      table_correct 8 h t8 /\
+      table_correct nzeros h tp /\
+      sub_table_correct (U32.v i) (nzeros + 8) h buf /\
+      B.live h t8 /\ B.live h tp)
+    (ensures fun h0 _ h1 -> 
+      M.modifies (B.loc_buffer buf) h0 h1 /\ table_correct (nzeros + 8) h1 buf) =
+    let open U32 in
+    let p = B.index tp i in
+    let j = p &^ 0xFFul in
+    UInt.logand_le (v p) (v 0xFFul);
+    let p' = B.index t8 j in
+    let p'' = p >>^ 8ul in
+    poly_mod_correct_eq nzeros i p;
+    poly_mod_correct_eq 8 j p';
+    large_table_val_aux i nzeros p p' p'';
+    buf.(i) <- p' ^^ p'';
+    if i <^ 255ul then gen_large_table nzeros (i +^ 1ul) t8 tp buf else ()
+    
+let gen_crc32_table t8 t16 t24 t32 =
+  gen_8bit_table 0ul t8;
+  gen_large_table 8 0ul t8 t8 t16;
+  gen_large_table 16 0ul t8 t16 t24;
+  gen_large_table 24 0ul t8 t24 t32
