specs/Spec.CRC32.fsti
@@ -1,89 +1,15 @@
 module Spec.CRC32
 
-module BV = FStar.BitVector
 module Seq = FStar.Seq
-module U8 = FStar.UInt8
-module U32 = FStar.UInt32
 
-unfold let gf2_plus (#n: nat{n > 0}) (a b: BV.bv_t n) : Tot (BV.bv_t n) =
-  BV.logxor_vec a b
-
-let (+@) #n = gf2_plus #n
-
-unfold let gf2_sub (#n: nat{n > 0}) (a b: BV.bv_t n) : Tot (BV.bv_t n) =
-  BV.logxor_vec a b
-
-let (-@) #n = gf2_sub #n
-
-let gf2_polynomial = Seq.init #bool 33 (fun i ->
-  i = 0 || i = 6 || i = 9 || i = 10 || i = 16 || i = 20 || i = 21 || i = 22 || i = 24 ||
-  i = 25 || i = 27 || i = 28 || i = 30 || i = 31 || i = 32)
-
-let gf2_polynomial32 = Seq.tail gf2_polynomial
-
-type crc32_polynomial = res: U32.t{
-  let res' = U32.v res in
-  forall i. UInt.nth res' i == Seq.index gf2_polynomial32 i
-}
-
-unfold let zero_vec_l (#n: nat{n > 0}) (m: nat) (a: BV.bv_t n): Tot (res: BV.bv_t (n + m){
+unfold let unsnoc (#a: Type) (s: Seq.seq a{
+  Seq.length s > 0
+}): Tot (res: Seq.seq a{
   forall i.
-    (i < m ==> Seq.index res i == false) /\
-    (i >= m /\ i < n + m ==> Seq.index res i == Seq.index a (i - m))
+    Seq.length res == Seq.length s - 1 /\
+    (Seq.index s i == Seq.index res i)
 }) =
-  match m with
-  | 0 -> a
-  | _ -> Seq.append (BV.zero_vec #m) a
+  Seq.slice s 0 (Seq.length s - 1)
 
-unfold let zero_vec_r (#n: nat{n > 0}) (m: nat) (a: BV.bv_t n): Tot (res: BV.bv_t (n + m){
-  forall i.
-    (i < n ==> Seq.index res i == Seq.index a i) /\ 
-    (i >= n /\ i < n + m ==> Seq.index res i == false)
-}) =
-  match m with
-  | 0 -> a
-  | _ -> Seq.append a (BV.zero_vec #m)
-
-unfold let ones_vec_l (#n: nat{n > 0}) (m: nat) (a: BV.bv_t n): Tot (res: BV.bv_t (n + m){
-  forall i.
-    (i < m ==> Seq.index res i == true) /\
-    (i >= m /\ i < n + m ==> Seq.index res i == Seq.index a (i - m))
-}) =
-  match m with
-  | 0 -> a
-  | _ -> Seq.append (BV.ones_vec #m) a
-
-unfold let ones_vec_r (#n: nat{n > 0}) (m: nat) (a: BV.bv_t n): Tot (res: BV.bv_t (n + m){
-  forall i.
-    (i < n ==> Seq.index res i == Seq.index a i) /\
-    (i >= n /\ i < n + m ==> Seq.index res i == true)
-}) =
-  match m with
-  | 0 -> a
-  | _ -> Seq.append a (BV.ones_vec #m)
-
-unfold let poly (n: nat{n >= 33}): Tot (p: BV.bv_t n{
-  Seq.index p (n - 1) == true
-}) =
-  zero_vec_l #33 (n - 33) gf2_polynomial
-
-unfold let poly_xor (#n: nat{n >= 32}) (a: BV.bv_t n): Tot (res: BV.bv_t n{
-  res == Seq.slice ((ones_vec_r 1 a) -@ poly (n + 1)) 0 n
-}) =
-  let a' = ones_vec_r 1 a in
-  let p = poly (n + 1) in
-  let r = a -@ (Seq.slice p 0 (Seq.length p - 1)) in
-  let r' = a' -@ p in
-  assert(Seq.equal r (Seq.slice r' 0 (Seq.length r' - 1)));
-  r
-
-let rec poly_mod (#n: nat{n > 32}) (a: BV.bv_t n): Tot (BV.bv_t 32) =
-  let p = poly n in
-  let b = if Seq.index a (n - 1) then a -@ p else a in
-  assert(Seq.index b (n - 1) == false);
-  if n = 33 then (Seq.slice b 0 (n - 1)) else poly_mod #(n - 1) (Seq.slice b 0 (n - 1))
-
-unfold let poly_mod_correct (d res: U32.t) =
-  let d' = zero_vec_l 1 (UInt.to_vec (U32.v d)) in
-  forall i. {:pattern UInt.nth (U32.v res) i}
-    UInt.nth (U32.v res) i == Seq.index (poly_mod d') i
+include Spec.CRC32.Bits
+include Spec.CRC32.Matrix
