code/Yazi.CRC32Table.fsti
@@ -1,0 +1,50 @@
+module Yazi.CRC32Table
+
+module B = LowStar.Buffer
+module CB = LowStar.ConstBuffer
+module Ghost = FStar.Ghost
+module HS = FStar.HyperStack
+module Spec = Spec.CRC32
+module M = LowStar.Modifies
+module ST = FStar.HyperStack.ST
+module U32 = FStar.UInt32
+
+type table_buf = buf: B.buffer U32.t{B.length buf == 256}
+
+private unfold let sub_table_correct
+  (j: nat{j <= 256})
+  (nzeros: nat{nzeros > 0})
+  (h: HS.mem)
+  (buf: table_buf) =
+  (B.live h buf) /\
+  (forall i. i < j ==>
+  Spec.poly_mod_correct nzeros (U32.uint_to_t i) (Seq.index (B.as_seq h buf) i))
+
+private unfold let table_correct
+  (nzeros: nat{nzeros > 0})
+  (h: HS.mem)
+  (buf: B.buffer U32.t{B.length buf == 256}) = sub_table_correct (B.length buf) nzeros h buf
+
+open LowStar.BufferOps
+
+val gen_crc32_table:
+    t8: table_buf
+  -> t16: table_buf
+  -> t24: table_buf
+  -> t32: table_buf
+  -> ST.Stack unit
+  (requires fun h ->
+    B.live h t8 /\ B.live h t16 /\ B.live h t24 /\ B.live h t32 /\
+    B.disjoint t8 t16 /\ B.disjoint t8 t24 /\ B.disjoint t8 t32 /\
+    B.disjoint t16 t24 /\ B.disjoint t16 t32 /\ B.disjoint t24 t32)
+  (ensures fun h0 _ h1 ->
+    M.modifies 
+      (B.loc_buffer t8 `B.loc_union`
+      B.loc_buffer t16 `B.loc_union`
+      B.loc_buffer t24 `B.loc_union`
+      B.loc_buffer t32)
+      h0 h1 /\
+    table_correct 8 h1 t8 /\
+    table_correct 16 h1 t16 /\
+    table_correct 24 h1 t24 /\
+    table_correct 32 h1 t32)
