specs/Spec.CRC32.Bits.fst
@@ -1,0 +1,252 @@
+module Spec.CRC32.Bits
+
+module BV = FStar.BitVector
+module Seq = FStar.Seq
+
+#set-options "--z3rlimit 200 --z3seed 1"
+let poly_xor_zero_prefix (#n: nat{n >= 32}) (a: BV.bv_t n) (m: nat{m > 0}): Lemma
+  (ensures forall (i: nat{i > 0}).
+    i < Seq.length (zero_vec_l m a) ==>
+    Seq.index (poly_xor (zero_vec_l m a)) i ==
+    Seq.index (poly_xor (zero_vec_l (m - 1) a)) (i - 1)) = ()
+
+let zero_vec_l_aux (#n: nat{n > 0}) (a: BV.bv_t n) (m: nat{m > 0}): Lemma
+  (ensures forall (i: nat{i > 0}).
+    i < Seq.length (zero_vec_l m a) ==>
+   Seq.index (zero_vec_l m a) i == Seq.index (zero_vec_l (m - 1) a) (i - 1)) = ()
+
+let rec poly_xor_zero_vec_l (#n: nat{n >= 32}) (a: BV.bv_t n) (m: nat): Lemma
+  (ensures zero_vec_l m (poly_xor a) == poly_xor (zero_vec_l m a)) =
+  match m with
+  | 0 -> ()
+  | _ ->
+    let b = zero_vec_l m (poly_xor a) in
+    let c = poly_xor (zero_vec_l m a) in
+    let b' = zero_vec_l (m - 1) (poly_xor a) in
+    let c' = poly_xor (zero_vec_l (m - 1) a) in
+    let p = poly (n + m + 1) in
+    let p' = unsnoc p in
+    poly_xor_zero_prefix a m;
+    zero_vec_l_aux (poly_xor a) m;
+    poly_xor_zero_vec_l a (m - 1);
+    calc (==) {
+      Seq.index c 0;
+      =={}
+      Seq.index ((zero_vec_l m a) -@ p') 0;
+      =={
+        assert(Seq.index (zero_vec_l m a) 0 == false);
+        assert(Seq.index p 0 == false);
+        assert(Seq.index p' 0 == false)
+      }
+      false;
+    };
+    assert(Seq.index b 0 == Seq.index c 0);
+    assert(Seq.equal b c)
+
+let poly_xor_sub_eq (#n: nat{n > 32}) (a: BV.bv_t n): Lemma
+  (ensures poly_xor #(n - 1) (unsnoc a) == unsnoc (a -@ (poly n))) =
+  assert(Seq.equal (poly_xor #(n - 1) (unsnoc a)) (unsnoc (a -@ (poly n))))
+
+let logxor_zero_eq (#n: nat{n > 0}) (a: BV.bv_t n): Lemma
+  (ensures (BV.logxor_vec a (BV.zero_vec #n)) == a)
+  [SMTPat (BV.logxor_vec a (BV.zero_vec #n))] =
+    let z = BV.zero_vec #n in
+    let x = BV.logxor_vec a z in
+    assert_norm(forall (i: nat) (v: BV.bv_t n). i < n ==> Seq.index v i = Seq.index v i <> false);
+    assert_norm(Seq.equal x a)
+
+let logxor_eq_zero (#n: nat{n > 0}) (a b: BV.bv_t n): Lemma
+  (requires a == b)
+  (ensures BV.logxor_vec a b == BV.zero_vec #n)
+  [SMTPat (BV.logxor_vec #n a b)] =
+  assert(Seq.equal (BV.logxor_vec a b) (BV.zero_vec #n))
+
+let rec logxor_vec_comm (#n: nat{n > 0}) (a b: BV.bv_t n): Lemma
+  (ensures BV.logxor_vec a b == BV.logxor_vec b a)
+  [SMTPat (BV.logxor_vec a b)] =
+  match n with
+  | 1 -> ()
+  | _ -> let c = BV.logxor_vec a b in
+    let c' = BV.logxor_vec b a in
+    assert_norm(Seq.index c 0 == Seq.index c' 0);
+    logxor_vec_comm #(n - 1) (Seq.tail a) (Seq.tail b)
+
+let logxor_vec_assoc (#n: nat{n > 0}) (a b c: BV.bv_t n): Lemma
+  (ensures BV.logxor_vec (BV.logxor_vec a b) c == BV.logxor_vec a (BV.logxor_vec b c))
+  [SMTPat (BV.logxor_vec (BV.logxor_vec a b) c); 
+   SMTPat (BV.logxor_vec a (BV.logxor_vec b c))] =
+  assert(Seq.equal (BV.logxor_vec (BV.logxor_vec a b) c) (BV.logxor_vec a (BV.logxor_vec b c)))
+
+let poly_xor_aux (#n: nat{n >= 32}) (a b: BV.bv_t n): Lemma
+  (ensures (poly_xor a) +@ (poly_xor b) == a +@ b) =
+  let p' = unsnoc (poly (n + 1)) in
+  calc (==) {
+    (poly_xor a) +@ (poly_xor b);
+    =={}
+    (a +@ p') +@ (b +@ p');
+    =={}
+    a +@ (p' +@ b +@ p');
+    =={}
+    a +@ (p' +@ p' +@ b);
+    =={}
+    a +@ b;
+  }
+
+let rec poly_mod_zero #n a =
+  match n with
+  | 33 -> assert_norm(Seq.equal (poly_mod #n a) (BV.zero_vec #32))
+  | _ -> 
+    assert_norm(Seq.equal (unsnoc a) (BV.zero_vec #(n - 1)));
+    poly_mod_zero #(n - 1) (unsnoc a)
+
+let rec poly_mod_add #n a b =
+  let a' = unsnoc a in
+  let b' = unsnoc b in
+  let c = a +@ b in
+  let c' = gf2_plus #(n - 1) a' b' in
+
+  if Seq.last a = Seq.last b then
+    assert(Seq.equal (unsnoc c) c')
+  else
+    assert(Seq.last a <> Seq.last b);
+
+  if n = 33 then begin
+    if Seq.last a then assert(Seq.equal (poly_mod a) (poly_xor #32 a')) else ();
+    if Seq.last b then assert(Seq.equal (poly_mod b) (poly_xor #32 b')) else ();
+    
+    match Seq.last a = Seq.last b with
+    | true -> if Seq.last a then poly_xor_aux #32 a' b' else ()
+    | false -> assert(Seq.equal (poly_mod c) (poly_xor c'))
+  end else begin
+    assert(n > 33);
+    if Seq.last a then begin
+      assert(Seq.equal (unsnoc (a -@ (poly n))) (poly_xor #(n - 1) a'));
+      assert_norm(poly_mod a == poly_mod (poly_xor #(n - 1) a'))
+    end else
+      assert_norm(poly_mod a == poly_mod #(n - 1) a');
+
+    if Seq.last b then begin
+      assert(Seq.equal (unsnoc (b -@ (poly n))) (poly_xor #(n - 1) b'));
+      assert_norm(poly_mod b == poly_mod (poly_xor #(n - 1) b'))
+    end else
+      assert_norm(poly_mod b == poly_mod #(n - 1) b');
+
+    match Seq.last a = Seq.last b with
+    | true ->
+      if Seq.last a then
+        let a'' = poly_xor #(n - 1) a' in
+        let b'' = poly_xor #(n - 1) b' in
+        calc (==) {
+          (poly_mod a) +@ (poly_mod b);
+          =={}
+          (poly_mod a'') +@ (poly_mod b'');
+          =={poly_mod_add a'' b''}
+          poly_mod (a'' +@ b'');
+          =={poly_xor_aux #(n - 1) a' b'}
+          poly_mod #(n - 1) (a' +@ b');
+          =={}
+          poly_mod c;
+        }
+      else
+        calc (==) {
+          (poly_mod a) +@ (poly_mod b);
+          =={}
+          (poly_mod #(n - 1) a') +@ (poly_mod #(n - 1) b');
+          =={poly_mod_add #(n - 1) a' b'}
+          poly_mod c';
+          =={}
+          poly_mod c;
+        }
+    | false ->
+      calc (==) {
+        poly_mod c;
+        =={assert(Seq.last c == true)}
+        poly_mod #(n - 1) (unsnoc (c -@ poly n));
+        =={assert(Seq.equal (unsnoc (c -@ poly n)) (poly_xor #(n - 1) c'))}
+        poly_mod (poly_xor #(n - 1) c');
+      };
+      let x = if Seq.last a then a else b in
+      let x' = unsnoc x in
+      let y = if Seq.last a then b else a in
+      let y' = unsnoc y in
+      let p' = unsnoc (poly n) in
+      calc (==) {
+        (poly_mod x) +@ (poly_mod y);
+        =={}
+        (poly_mod (poly_xor #(n - 1) x')) +@ (poly_mod #(n - 1) y');
+        =={poly_mod_add #(n - 1) (poly_xor #(n - 1) x') y'}
+        poly_mod ((poly_xor #(n - 1) x') +@ y');
+        =={}
+        poly_mod c;
+      }
+  end
+
+let rec poly_mod_zero_prefix #n a m =
+  assert(Seq.equal (zero_vec_l #(n - 1) m (unsnoc a)) (unsnoc (zero_vec_l m a)));
+  if n = 33 then
+    if Seq.index a (n - 1) then
+      calc (==) {
+        poly_mod (zero_vec_l m (poly_mod a));
+        =={assert(Seq.equal (poly_mod a) (poly_xor #(n - 1) (unsnoc a)))}
+        poly_mod (zero_vec_l m (poly_xor #(n - 1) (unsnoc a)));
+        =={
+          let left = (zero_vec_l m (poly_xor #(n - 1) (unsnoc a))) in
+          let right = (poly_xor #(n + m - 1) (unsnoc (zero_vec_l m a))) in
+          assert(Seq.equal left right)
+        }
+        poly_mod (poly_xor #(n + m - 1) (unsnoc (zero_vec_l m a)));
+        =={poly_xor_sub_eq (zero_vec_l m a)}
+        poly_mod (zero_vec_l m a);
+      }
+    else
+      calc (==) {
+        poly_mod (zero_vec_l m (poly_mod a));
+        =={}
+        poly_mod (zero_vec_l #(n - 1) m (unsnoc a));
+        =={}
+        poly_mod #(n + m - 1) (unsnoc (zero_vec_l m a));
+        =={}
+        poly_mod (zero_vec_l m a);
+      }
+  else
+    if Seq.index a (n - 1) then
+      calc (==) {
+        poly_mod (zero_vec_l m (poly_mod a));
+        =={}
+        poly_mod (zero_vec_l m (poly_mod #(n - 1) (unsnoc (a -@ (poly n)))));
+        =={poly_xor_sub_eq a}
+        poly_mod (zero_vec_l m (poly_mod (poly_xor #(n - 1) (unsnoc a))));
+        =={poly_mod_zero_prefix (poly_xor #(n - 1) (unsnoc a)) m}
+        poly_mod (zero_vec_l m (poly_xor #(n - 1) (unsnoc a)));
+        =={poly_xor_zero_vec_l #(n - 1) (unsnoc a) m}
+        poly_mod (poly_xor (zero_vec_l #(n - 1) m (unsnoc a)));
+        =={}
+        poly_mod (poly_xor #(n + m - 1) (unsnoc (zero_vec_l m a)));
+        =={poly_xor_sub_eq (zero_vec_l m a)}
+        poly_mod #(n + m - 1) (unsnoc ((zero_vec_l m a) -@ poly (n + m)));
+        =={assert(Seq.last (zero_vec_l m a) == true)}
+        poly_mod (zero_vec_l m a);
+      }
+    else
+      calc (==) {
+        poly_mod (zero_vec_l m (poly_mod a));
+        =={}
+        poly_mod (zero_vec_l m (poly_mod #(n - 1) (unsnoc a)));
+        =={poly_mod_zero_prefix #(n - 1) (unsnoc a) m}
+        poly_mod (zero_vec_l #(n - 1) m (unsnoc a));
+        =={}
+        poly_mod #(n + m - 1) (unsnoc (zero_vec_l m a));
+        =={}
+        poly_mod (zero_vec_l m a);
+      }
+
+let rec poly_mod_zero_suffix a m =
+  match m with
+  | 1 -> assert(Seq.equal (poly_mod (zero_vec_r m a)) a)
+  | _ ->
+    calc (==) {
+      poly_mod (zero_vec_r m a);
+      =={assert(Seq.equal (unsnoc (zero_vec_r m a)) (zero_vec_r (m - 1) a))}
+      poly_mod (zero_vec_r (m - 1) a);
+    };
+    poly_mod_zero_suffix a (m - 1)
