specs/Spec.CRC32.Bits.fsti
@@ -1,0 +1,124 @@
+module Spec.CRC32.Bits
+module BV = FStar.BitVector
+module Seq = FStar.Seq
+module U32 = FStar.UInt32
+module UInt = FStar.UInt
+
+unfold let zero_vec_l (#n: nat{n > 0}) (m: nat) (a: BV.bv_t n): Tot (res: BV.bv_t (n + m){
+  forall i.
+    (i < m ==> Seq.index res i == false) /\
+    (i >= m /\ i < n + m ==> Seq.index res i == Seq.index a (i - m))
+}) =
+  match m with
+  | 0 -> a
+  | _ -> Seq.append (BV.zero_vec #m) a
+
+unfold let zero_vec_r (#n: nat{n > 0}) (m: nat) (a: BV.bv_t n): Tot (res: BV.bv_t (n + m){
+  forall i.
+    (i < n ==> Seq.index res i == Seq.index a i) /\ 
+    (i >= n /\ i < n + m ==> Seq.index res i == false)
+}) =
+  match m with
+  | 0 -> a
+  | _ -> Seq.append a (BV.zero_vec #m)
+
+unfold let ones_vec_l (#n: nat{n > 0}) (m: nat) (a: BV.bv_t n): Tot (res: BV.bv_t (n + m){
+  forall i.
+    (i < m ==> Seq.index res i == true) /\
+    (i >= m /\ i < n + m ==> Seq.index res i == Seq.index a (i - m))
+}) =
+  match m with
+  | 0 -> a
+  | _ -> Seq.append (BV.ones_vec #m) a
+
+unfold let ones_vec_r (#n: nat{n > 0}) (m: nat) (a: BV.bv_t n): Tot (res: BV.bv_t (n + m){
+  forall i.
+    (i < n ==> Seq.index res i == Seq.index a i) /\
+    (i >= n /\ i < n + m ==> Seq.index res i == true)
+}) =
+  match m with
+  | 0 -> a
+  | _ -> Seq.append a (BV.ones_vec #m)
+
+let zero_vec_l_app (#n: nat{n > 0}) (a: BV.bv_t n) (m l: nat): Lemma
+  (ensures zero_vec_l l (zero_vec_l m a) == zero_vec_l (m + l) a) =
+  assert(Seq.equal (zero_vec_l l (zero_vec_l m a)) (zero_vec_l (m + l) a))
+
+unfold let gf2_plus (#n: nat{n > 0}) (a b: BV.bv_t n) : Tot (BV.bv_t n) =
+  BV.logxor_vec a b
+
+let (+@) #n = gf2_plus #n
+
+unfold let gf2_sub (#n: nat{n > 0}) (a b: BV.bv_t n) : Tot (BV.bv_t n) =
+  BV.logxor_vec a b
+
+let (-@) #n = gf2_sub #n
+
+unfold let unsnoc (#a: Type) (s: Seq.seq a{
+  Seq.length s > 0
+}): Tot (res: Seq.seq a{
+  forall i.
+    Seq.length res == Seq.length s - 1 /\
+    (Seq.index s i == Seq.index res i)
+}) =
+  Seq.slice s 0 (Seq.length s - 1)
+
+let gf2_polynomial = Seq.init #bool 33 (fun i ->
+  i = 0 || i = 6 || i = 9 || i = 10 || i = 16 || i = 20 || i = 21 || i = 22 || i = 24 ||
+  i = 25 || i = 27 || i = 28 || i = 30 || i = 31 || i = 32)
+
+let gf2_polynomial32 = unsnoc gf2_polynomial
+
+type crc32_polynomial = res: U32.t{
+  let res' = U32.v res in
+  forall i. UInt.nth res' i == Seq.index gf2_polynomial32 i
+}
+
+unfold let poly (n: nat{n >= 33}): Tot (p: BV.bv_t n{
+  Seq.index p (n - 1) == true
+}) =
+  assert(Seq.index gf2_polynomial 31 == true);
+  zero_vec_l #33 (n - 33) gf2_polynomial
+
+unfold let poly_xor (#n: nat{n >= 32}) (a: BV.bv_t n): Tot (res: BV.bv_t n{
+  res == unsnoc ((ones_vec_r 1 a) -@ poly (n + 1))
+}) =
+  let a' = ones_vec_r 1 a in
+  let p = poly (n + 1) in
+  let r = a -@ (unsnoc p) in
+  let r' = a' -@ p in
+  assert(Seq.equal r (unsnoc r'));
+  r
+
+let rec poly_mod (#n: nat{n > 32}) (a: BV.bv_t n): Tot (BV.bv_t 32) =
+  let p = poly n in
+  let b = if Seq.index a (n - 1) then a -@ p else a in
+  assert(Seq.index b (n - 1) == false);
+  if n = 33 then unsnoc b else poly_mod #(n - 1) (unsnoc b)
+
+val poly_mod_zero: #n: nat{n > 32} -> a: BV.bv_t n {a == BV.zero_vec #n} -> Lemma
+  (ensures poly_mod a == BV.zero_vec #32)
+
+val poly_mod_add: #n: nat{n > 32} -> a: BV.bv_t n ->  b: BV.bv_t n -> Lemma
+  (ensures (poly_mod a) +@ (poly_mod b) == poly_mod (a +@ b))
+
+val poly_mod_zero_prefix: #n: nat{n > 32} -> a: BV.bv_t n -> m: nat{m > 0} -> Lemma
+  (ensures poly_mod (zero_vec_l m (poly_mod a)) == poly_mod (zero_vec_l m a))
+
+val poly_mod_zero_suffix: a: BV.bv_t 32 -> m: nat{m > 0} -> Lemma
+  (ensures poly_mod (zero_vec_r m a) == a)
+
+unfold let poly_mod_correct (nzeros: nat{nzeros > 0}) (d res: U32.t) =
+  let d' = zero_vec_l nzeros (UInt.to_vec (U32.v d)) in
+  forall i. {:pattern UInt.nth (U32.v res) i}
+    UInt.nth (U32.v res) i == Seq.index (poly_mod d') i
+
+unfold let poly_mod_u32 (nzeros: nat{nzeros > 0}) (d: U32.t) =
+  poly_mod (zero_vec_l nzeros (UInt.to_vec (U32.v d)))
+
+let poly_mod_correct_eq (nzeros: nat{nzeros > 0}) (d res: U32.t): Lemma
+  (requires poly_mod_correct nzeros d res)
+  (ensures poly_mod_u32 nzeros d == UInt.to_vec (U32.v res)) =
+  let open U32 in
+  assert(forall i. UInt.nth (v res) i == Seq.index (UInt.to_vec (v res)) i);
+  assert(Seq.equal (poly_mod (zero_vec_l nzeros (UInt.to_vec (U32.v d)))) (UInt.to_vec (v res)))
