specs/Spec.CRC32.Matrix.fst
@@ -1,0 +1,206 @@
+module Spec.CRC32.Matrix
+
+module BV = FStar.BitVector
+module Bits = Spec.CRC32.Bits
+module Seq = FStar.Seq
+
+open FStar.Seq
+open FStar.Mul
+open Spec.CRC32.Bits
+
+let rec seq_append_index_r (#t: Type) (a b: Seq.seq t): Lemma
+  (ensures forall i. i < Seq.length b ==> Seq.index (a @| b) (i + Seq.length a) == Seq.index b i)
+  (decreases Seq.length a) =
+  match Seq.length a with
+  | 0 -> ()
+  | _ -> seq_append_index_r (Seq.tail a) b
+
+val magic_matrix_init: s: sub_matrix_t 1 -> Tot (matrix_t 1) (decreases 32 - (Seq.length s))
+
+let rec magic_matrix_init s =
+  let l = Seq.length s in
+  if l = 0 then begin
+    let m = ones_vec_r 1 (BV.zero_vec #32) in
+    let n = poly_xor (BV.zero_vec #32) in
+    calc (==) {
+      poly_mod #33 m;
+      =={assert(last m == true)}
+      unsnoc (m -@ poly 33);
+      =={}
+      n;
+    };
+    let res = s @| (Seq.create 1 n) in
+    calc (==) {
+      Seq.index res l;
+      =={seq_append_index_r s (Seq.create 1 n)}
+      Seq.index (Seq.create 1 n) 0;
+      =={}
+      n;
+    };
+    magic_matrix_init res
+  end else if l < 32 then begin
+    let n = magic_matrix_pattern 1 l in
+    let res = s @| (Seq.create 1 (poly_mod n)) in
+    calc (==) {
+      Seq.index res l;
+      =={seq_append_index_r s (Seq.create 1 (poly_mod n))}
+      Seq.index (Seq.create 1 (poly_mod n)) 0;
+      =={}
+      poly_mod n;
+    };
+    magic_matrix_init res
+  end else 
+    s
+
+type matrix_dividend (nzeros: nat{nzeros > 0}) = d: BV.bv_t (nzeros + 32) {
+  forall i. i < nzeros ==> Seq.index d i == false
+}
+
+val bit_extract:
+    #nzeros: nat{nzeros > 0}
+  -> n: matrix_dividend nzeros
+  -> i: nat{i < 32}
+  -> res: BV.bv_t (nzeros + 32) {
+      forall j.
+        (j == nzeros + 31 - i ==> Seq.index res j == Seq.index n j) /\
+        (j <> nzeros + 31 - i ==> Seq.index res j == false)
+    }
+
+let bit_extract #nzeros n i =
+  let zero_left = BV.zero_vec #(nzeros + 32 - i - 1) in
+  let bit = zero_left @| (Seq.create 1 (Seq.index n (nzeros + 31 - i))) in
+  zero_vec_r #(nzeros + 32 - i) i bit
+
+val bit_sum:
+    #nzeros: nat{nzeros > 0}
+  -> n: matrix_dividend nzeros
+  -> i: nat{i < 32}
+  -> res: BV.bv_t (nzeros + 32) {
+    forall j.
+      (j >= nzeros + 31 - i ==> Seq.index res j == Seq.index n j) /\
+      (j < nzeros + 31 - i ==> Seq.index res j == false)
+  }
+
+let rec bit_sum #nzeros n i =
+  match i with
+  | 0 -> bit_extract #nzeros n i
+  | _ -> (bit_extract n i) +@ (bit_sum n (i - 1))
+
+val do_magic_matrix_times:
+    #nzeros: nat{nzeros > 0}
+  -> m: matrix_t nzeros
+  -> n: BV.bv_t 32
+  -> i: nat{i < 32}
+  -> res: BV.bv_t 32{
+      res == poly_mod (bit_extract #nzeros (zero_vec_l nzeros n) i)
+    }
+
+let do_magic_matrix_times #nzeros m n i =
+  let pat = magic_matrix_pattern nzeros i in
+  let ext = bit_extract #nzeros (zero_vec_l nzeros n) i in
+  if Seq.index n (31 - i) then begin
+    Seq.index m i
+  end else begin
+    assert(Seq.equal ext (BV.zero_vec #(nzeros + 32)));
+    Bits.poly_mod_zero ext;
+    BV.zero_vec #32
+  end
+
+val magic_matrix_times':
+    #nzeros: nat{nzeros > 0}
+  -> m: matrix_t nzeros
+  -> n: BV.bv_t 32
+  -> i: nat{i < 32}
+  -> res: BV.bv_t 32{
+    res == poly_mod (bit_sum #nzeros (zero_vec_l nzeros n) i)
+  }
+
+let rec magic_matrix_times'
+  (#nzeros: nat{nzeros > 0}) (m: matrix_t nzeros) (n: BV.bv_t 32) (i: nat{i < 32}) =
+  match i with
+  | 0 -> do_magic_matrix_times m n i
+  | _ -> 
+    let n' = do_magic_matrix_times m n i in
+    let e = bit_extract #nzeros (zero_vec_l nzeros n) i in
+    let sum = bit_sum #nzeros (zero_vec_l nzeros n) (i - 1) in
+    Bits.poly_mod_add e sum;
+    n' +@ magic_matrix_times' m n (i - 1)
+
+val magic_matrix_times:
+  #nzeros: nat {nzeros > 0} ->
+  matrix_t nzeros ->
+  n: BV.bv_t 32 ->
+  res: BV.bv_t 32 {res == poly_mod (zero_vec_l nzeros n)}
+
+let magic_matrix_times #nzeros m n =
+  assert(Seq.equal (bit_sum #nzeros (zero_vec_l nzeros n) 31) (zero_vec_l nzeros n));
+  magic_matrix_times' m n 31
+
+#set-options "--z3rlimit 200 --z3seed 1"
+
+
+let magic_matrix_times_double
+  (#nzeros: nat{nzeros > 0}) (m: matrix_t nzeros) (i: nat{i < 32}): Lemma
+  (ensures is_magic_matrix_elem (nzeros * 2) i (magic_matrix_times m (Seq.index m i))) =
+  let p = magic_matrix_pattern nzeros i in
+  let p' = magic_matrix_pattern (nzeros * 2) i in
+  let p'' = zero_vec_l nzeros p in
+  let n = magic_matrix_times m (Seq.index m i) in
+  poly_mod_zero_prefix p nzeros;
+  assert(forall j.
+    j >= nzeros /\ j < nzeros * 2 + 32 ==>
+    Seq.index p (j - nzeros) == Seq.index p' j /\
+    Seq.index p (j - nzeros) == Seq.index p'' j);
+  assert(forall j. j < nzeros ==> Seq.index p' j == Seq.index p'' j);
+  assert(Seq.equal p'' p');
+  calc (==) {
+    n;
+    =={}
+    poly_mod (zero_vec_l nzeros (Seq.index m i));
+    =={}
+    poly_mod (zero_vec_l nzeros (poly_mod p));
+    =={}
+    poly_mod (zero_vec_l nzeros p);
+    =={}
+    poly_mod p';
+    =={}
+    poly_mod (magic_matrix_pattern (nzeros * 2) i);
+  }
+
+val magic_matrix_square':
+    #nzeros: nat{nzeros > 0}
+  -> m: matrix_t nzeros
+  -> s: sub_matrix_t (nzeros * 2)
+  -> Tot (matrix_t (nzeros * 2))
+    (decreases 32 - (Seq.length s))
+
+let rec magic_matrix_square' #nzeros m s =
+  if Seq.length s < 32 then begin
+    magic_matrix_times_double m (Seq.length s);
+    let n = magic_matrix_times m (Seq.index m (Seq.length s)) in
+    let res = s @| (Seq.create 1 n) in
+    seq_append_index_r s (Seq.create 1 n);
+    calc (==) {
+      poly_mod (magic_matrix_pattern (nzeros * 2) (Seq.length s));
+      =={}
+      n;
+      =={}
+      Seq.index (Seq.create 1 n) 0;
+      =={}
+      Seq.index res (Seq.length s);
+    };
+    assert(forall i.{:pattern Seq.index res i}
+      i < Seq.length s ==> Seq.index res i == Seq.index s i);
+    assert(forall i. i < Seq.length res ==> is_magic_matrix_elem (nzeros * 2) i (Seq.index res i));
+    magic_matrix_square' #nzeros m res
+  end
+  else
+    s
+
+val magic_matrix_square:
+    #nzeros: nat {nzeros > 0}
+  -> matrix_t nzeros
+  -> Tot (matrix_t (nzeros * 2))
+
+let magic_matrix_square #_ m =
+  magic_matrix_square' m (Seq.empty #(BV.bv_t 32))
