specs/Spec.CRC32.Matrix.fsti
@@ -1,0 +1,26 @@
+module Spec.CRC32.Matrix
+
+module BV = FStar.BitVector
+module Seq = FStar.Seq
+module Bits = Spec.CRC32.Bits
+
+let magic_matrix_pattern (nzeros: nat{nzeros > 0}) (i: nat{i < 32}):
+  res: BV.bv_t (nzeros + 32){
+    forall j.
+      (j == nzeros + 31 - i ==> Seq.index res j == true) /\
+      (j <> nzeros + 31 - i ==> Seq.index res j == false)
+  } =
+  let zero_left = BV.zero_vec #(nzeros + 32 - i - 1) in
+  let one = Bits.ones_vec_r 1 zero_left in
+  Bits.zero_vec_r i one
+
+let is_magic_matrix_elem (nzeros: nat{nzeros > 0}) (i: nat {i < 32}) (v: BV.bv_t 32) =
+  Bits.poly_mod (magic_matrix_pattern nzeros i) == v
+
+type matrix_seq = s:Seq.seq (BV.bv_t 32) {Seq.length s <= 32}
+
+type sub_matrix_t (nzeros: nat{nzeros > 0}) = m: matrix_seq{
+   forall i. i < Seq.length m ==> is_magic_matrix_elem nzeros i (Seq.index m i)
+}
+
+type matrix_t (nzeros: nat{nzeros > 0}) = m: sub_matrix_t nzeros{Seq.length m == 32}
